theories/zoo/iris/base_logic/lib/saved_prop.v
@@ -31,6 +31,11 @@ Section saved_prop_G.
   Definition saved_prop γ P :=
     agree_on γ (Next P).
 
+  #[global] Instance saved_prop_contractive γ :
+    Contractive (saved_prop γ).
+  Proof.
+    solve_contractive.
+  Qed.
   #[global] Instance saved_prop_proper γ :
     Proper ((≡) ==> (≡)) (saved_prop γ).
   Proof.
